Start adding multiret to dataLang

compiler/backend/semantics/dataSemScript.sml
@@ -1277,6 +1277,10 @@ Definition dest_thunk_def:
   dest_thunk v refs = NotThunk
 End
 
+Definition set_vars_def:
+  set_vars ns vs s = (s with locals := union (fromAList (ZIP (ns,vs))) s.locals)
+End
+
 Definition evaluate_def:
   (evaluate (Skip,^s) = (NONE,s)) /\
   (evaluate (Move dest src,s) =
@@ -1311,10 +1315,10 @@ Definition evaluate_def:
        (case jump_exc s of
         | NONE => (SOME (Rerr(Rabort Rtype_error)),s)
         | SOME s => (SOME (Rerr(Rraise x)),s))) /\
-  (evaluate (Return n,s) =
-     case get_var n s.locals of
+  (evaluate (Return ns,s) =
+     case get_vars ns s.locals of
      | NONE => (SOME (Rerr(Rabort Rtype_error)),s)
-     | SOME x => (SOME (Rval x),flush_state F s)) /\
+     | SOME xs => (SOME (Rval xs),flush_state F s)) /\
   (evaluate (Seq c1 c2,s) =
      let (res,s1) = fix_clock s (evaluate (c1,s)) in
        if res = NONE then evaluate (c2,s1) else (res,s1)) /\
@@ -1334,7 +1338,7 @@ Definition evaluate_def:
         | NotThunk => (SOME (Rerr (Rabort Rtype_error)),s)
         | IsThunk Evaluated v =>
           (case ret of
-           | NONE => (SOME (Rval v),flush_state F s)
+           | NONE => (SOME (Rval [v]),flush_state F s)
            | SOME (dest,names) =>
              (case cut_env names s.locals of
               | NONE => (SOME (Rerr(Rabort Rtype_error)),s)
@@ -1362,10 +1366,13 @@ Definition evaluate_def:
                            s1 with <| stack := [] ; locals := LN |>)
                         else
                           (case fix_clock s1 (evaluate (prog, s1)) of
-                           | (SOME (Rval x),s2) =>
-                             (case pop_env s2 of
-                              | NONE => (SOME (Rerr(Rabort Rtype_error)),s2)
-                              | SOME s1 => (NONE, set_var dest x s1))
+                           | (SOME (Rval xs),s2) =>
+                             (if LENGTH xs = 1 then
+                                case pop_env s2 of
+                                | NONE => (SOME (Rerr(Rabort Rtype_error)),s2)
+                                | SOME s1 => (NONE, set_var dest (HD xs) s1)
+                              else
+                                (SOME (Rerr(Rabort Rtype_error)),s2))
                            | (NONE,s) => (SOME (Rerr(Rabort Rtype_error)),s)
                            | res => res)))))) /\
   (evaluate (Call ret dest args handler,s) =
@@ -1386,7 +1393,7 @@ Definition evaluate_def:
                   | (NONE,s) => (SOME (Rerr(Rabort Rtype_error)),s)
                   | (SOME res,s) => (SOME res,s))
                else (SOME (Rerr(Rabort Rtype_error)),s)
-           | SOME (n,names) (* returning call, returns into var n *) =>
+           | SOME (ns,names) (* returning call, returns into var n *) =>
              (case cut_env names s.locals of
               | NONE => (SOME (Rerr(Rabort Rtype_error)),s)
               | SOME env =>
@@ -1396,10 +1403,13 @@ Definition evaluate_def:
                    then (SOME (Rerr(Rabort Rtimeout_error)),
                         s1 with <| stack := [] ; locals := LN |>)
                    else (case fix_clock s1 (evaluate (prog, s1)) of
-                         | (SOME (Rval x),s2) =>
-                           (case pop_env s2 of
-                            | NONE => (SOME (Rerr(Rabort Rtype_error)),s2)
-                            | SOME s1 => (NONE, set_var n x s1))
+                         | (SOME (Rval xs),s2) =>
+                           (if LENGTH xs = LENGTH ns ∧ ALL_DISTINCT ns then
+                              (case pop_env s2 of
+                               | NONE => (SOME (Rerr(Rabort Rtype_error)),s2)
+                               | SOME s1 => (NONE, set_vars ns xs s1))
+                            else
+                              (SOME (Rerr(Rabort Rtype_error)),s2))
                          | (SOME (Rerr(Rraise x)),s2) =>
                            (* if handler is present, then handle exc *)
                            (case handler of
@@ -1465,8 +1475,14 @@ Proof
   \\ rw[do_stack_clock]
 QED
 
+Theorem set_vars_clock[local,simp]:
+  (set_vars ns vs s).clock = s.clock
+Proof
+  simp [set_vars_def]
+QED
+
 Theorem evaluate_clock:
- !xs s1 vs s2. (evaluate (xs,s1) = (vs,s2)) ==> s2.clock <= s1.clock
+  !xs s1 vs s2. (evaluate (xs,s1) = (vs,s2)) ==> s2.clock <= s1.clock
 Proof
   recInduct evaluate_ind >> rw[evaluate_def] >>
   every_case_tac >>
